books/centaur/misc/make-list.lisp
@@ -1,0 +1,16 @@
+
+(in-package "ACL2")
+
+;; This simply provides a non-tail-recursive way of reasoning about
+;; make-list-ac, which is the macroexpansion of make-list.
+
+(defthm make-list-ac-redef
+  (equal (make-list-ac n val ac)
+         (if (zp n)
+             ac
+           (cons val (make-list-ac (1- n) val ac))))
+  :rule-classes ((:definition
+                  :clique (make-list-ac)
+                  :controller-alist ((make-list-ac t nil nil)))))
+
+(in-theory (disable make-list-ac))
